Core/Traces.v
@@ -1,16 +1,17 @@
 From Coq Require Import
-    List
-    Relations
-    Init.Nat.
+  List
+  Relations
+  Init.Nat.
 
 From LHL.Util Require Import
-    Util
-    ListUtil
-    TransUtil.
+  Util
+  ListUtil
+  TransUtil.
 
 From LHL.Core Require Import
-    Program
-    Specs.
+  Program
+  Specs
+  Eutt.
 
 Set Implicit Arguments.
 Set Contextual Implicit.
@@ -21,49 +22,37 @@ Unset Strict Implicit.
 Definition Trace (T : Type) : Type := list T.
 
 Definition PrefixOf {T} (ρ σ : Trace T) : Prop :=
-    exists τ, σ = app ρ τ.
+  exists τ, σ = app ρ τ.
 
 Definition projAgentEv {A} i (ev : nat * A) : option (nat * A) :=
-    if eqb (fst ev) i then
-        Some ev
-    else
-        None.
+  if eqb (fst ev) i then
+    Some ev
+  else
+    None.
 
 Definition projOverEv {E F : ESig} (ev : @ThreadLEvent E F) : option (ThreadEvent F) := 
-    match ev with
-    | (i, OCallEv m) => Some (i, CallEv m)
-    | (i, ORetEv m n) => Some (i, RetEv m n)
-    | (_, UCallEv _) => None
-    | (_, URetEv _ _) => None
-    | (_, Silent) => None
-    end.
+  match ev with
+  | (i, OEvent ev) => Some (i, ev)
+  | _ => None
+  end.
 
 Definition projUnderEv {E F : ESig} (ev : @ThreadLEvent E F) : option (ThreadEvent E) := 
-    match ev with
-    | (_, OCallEv _) => None
-    | (_, ORetEv _ _) => None
-    | (i, UCallEv m) => Some (i, CallEv m)
-    | (i, URetEv m n) => Some (i, RetEv m n)
-    | (_, Silent) => None
-    end.
+  match ev with
+  | (i, UEvent (Some ev)) => Some (i, ev)
+  | _ => None
+  end.
 
 Definition liftUEv {E F} (ev : @Event E) : @LEvent E F :=
-    match ev with
-    | CallEv m => UCallEv m
-    | RetEv m v => URetEv m v
-    end.
+  UEvent (Some ev).
 
 Definition liftOEv {E F} (ev : @Event F) : @LEvent E F :=
-    match ev with
-    | CallEv m => OCallEv m
-    | RetEv m v => ORetEv m v
-    end.
+  OEvent ev.
 
 Notation projOver := (mapfilter projOverEv).
 Notation projUnder := (mapfilter projUnderEv).
 Definition projAgent {A} i : 
-    Trace (ThreadName * A) -> Trace (ThreadName * A) := 
-        (mapfilter (projAgentEv i)).
+  Trace (ThreadName * A) -> Trace (ThreadName * A) := 
+    (mapfilter (projAgentEv i)).
 Notation liftU := (map liftUEv).
 Notation liftO := (map liftOEv).
 
@@ -71,157 +60,109 @@ Notation liftO := (map liftOEv).
 
 Inductive ThreadState {E F : ESig} : Type :=
 | Idle
-| Cont {Ret} (m : F Ret) (p : Prog E Ret) 
-| UCall {Ret A} (m : F Ret) (k : A -> Prog E Ret)
-.
+| Cont {A} (m : F A) (p : Prog E A) 
+| UCall {A B} (m : F A) (k : A -> Prog E B).
+Arguments ThreadState : clear implicits.
 
-Definition ThreadsSt {E F : ESig} : Type := ThreadName -> ThreadState (E := E) (F := F).
+Definition ThreadsSt (E F : ESig) : Type := ThreadName -> ThreadState E F.
 
-Definition updt_thst {E F : ESig} := 
-    updt_istate (A := ThreadName) (State :=ThreadState (E := E) (F := F))  (eqA := eqb).
+Definition updt_thst (E F : ESig) := 
+  @updt_istate ThreadName (ThreadState E F) eqb.
 
-Definition allIdle {E F : ESig} : ThreadsSt (E := E) (F := F) := fun n => Idle.
+Definition allIdle {E F : ESig} : ThreadsSt E F := fun n => Idle.
 
-Definition ThreadStep {E F : ESig}
-    (M : Impl E F) (th : ThreadState) (e : LEvent E F) (th' : ThreadState) : Prop :=
-        match e with 
-        | @OCallEv _ _ R m => th = Idle /\ th' = Cont m (M R m)
-        | @ORetEv _ _ R m n => th = Cont m (Return n) /\ th' = Idle
-        | @UCallEv _ _ A m => exists R m' (k : _ -> _ R), th = Cont m' (Bind m k) /\ th' = UCall m' (A := A) k
-        | @URetEv _ _ A _ n =>  exists R m (k : _ -> _ R), th = UCall m k /\ th' = Cont m (k n)
-        | Silent => exists R m (p : _ R), th = Cont m (NoOp p) /\ th' = Cont m p
-        end.
+Variant OverThreadStep {E F : ESig} (M : Impl E F) :
+  ThreadState E F -> Event F -> ThreadState E F -> Prop :=
+| OCallThreadStep th th' A (m : F A) C :
+  th = Idle ->
+  eutt ieq (M _ m) C ->
+  th' = Cont m C ->
+  OverThreadStep M th (CallEv m) th'
+| ORetThreadStep th th' A (m : F A) v :
+  th = Cont m (Return v) ->
+  th' = Idle ->
+  OverThreadStep M th (RetEv m v) th'.
+
+Variant UnderThreadStep {E F : ESig} :
+  ThreadState E F -> option (Event E) -> ThreadState E F -> Prop :=
+| UCallThreadStep A th th' (um : E A) om k :
+  th = Cont om (Bind um k) ->
+  th' = UCall om k ->
+  UnderThreadStep th (Some (CallEv um)) th'
+| URetThreadStep A th th' (um : E A) om v k :
+  th = UCall om k ->
+  th' = Cont om (k v) ->
+  UnderThreadStep th (Some (RetEv um v)) th'
+| USilentThreadStep A th th' om (p : Prog E A) :
+  th = Cont om (NoOp p) ->
+  th' = Cont om p ->
+  UnderThreadStep th None th'.
+
+Variant ThreadStep {E F : ESig} (M : Impl E F) :
+  ThreadState E F -> LEvent E F -> ThreadState E F -> Prop :=
+| UThreadStep th e th' :
+  UnderThreadStep th e th' ->
+  ThreadStep M th (UEvent e) th'
+| OThreadStep th e th' :
+  OverThreadStep M th e th' ->
+  ThreadStep M th (OEvent e) th'.
 
 Definition ThreadsStep E F (M : Impl E F)
-  : ThreadsSt -> ThreadLEvent E F -> ThreadsSt -> Prop :=
+  : ThreadsSt E F -> ThreadLEvent E F -> ThreadsSt E F -> Prop :=
   PointStep (ThreadStep (E := E) M).
-
-Definition ThreadsSteps {E F} (M : Impl E F)
-  : ThreadsSt -> Trace (ThreadLEvent E F) -> ThreadsSt -> Prop :=
-  Steps (ThreadsStep M).
 
 (* Trace Semantics *)
 
 Definition IsTraceOfImpl {E F : ESig} (t : Trace (ThreadLEvent E F)) (M : Impl E F) : Prop :=
-    exists thst, IsPathOf allIdle t thst (ThreadsSteps M).
-    
+  exists thst, Steps (ThreadsStep M) allIdle t thst.
+  
 Definition IsTraceOfSpec {E : ESig} (t : Trace (ThreadEvent E)) (spec : Spec E) : Prop := 
-    exists st, IsPathOf spec.(Init) t st (Steps spec.(Step)).
+  exists st, Steps spec.(Step) spec.(Init) t st.
 
 Definition IsTraceOfLayer {E F : ESig} (t : Trace (ThreadLEvent E F)) (lay : @Layer E F) : Prop :=
-    IsTraceOfSpec (projUnder t) lay.(USpec) /\ IsTraceOfImpl t lay.(LImpl).
-
-Definition IsTraceOfOver {E F : ESig} (t : Trace (ThreadEvent F)) (lay : @Layer E F) : Prop :=
-    exists t', t = projOver t' /\ IsTraceOfLayer t' lay.
+  IsTraceOfSpec (projUnder t) lay.(USpec) /\ IsTraceOfImpl t lay.(LImpl).
 
 (* Interactions *)
 
-Definition InterState {E F : ESig} {spec : Spec E} : Type :=
-    (ThreadsSt (E := E) (F := F)) * spec.(State).
+Definition InterState {E : ESig} F (spec : Spec E) : Type :=
+  ThreadsSt E F * spec.(State).
 
-Definition updThs {A} (ths : ThreadName -> A) i (st : A) : ThreadName -> A :=
-    fun j =>
-        if eqb i j then
-            st
-        else
-            ths j.
+Definition InterUStep {E F : ESig} {spec : Spec E} (i : ThreadName)
+  (s : InterState F spec)
+  (ev : option (Event E))
+  (t : InterState F spec) :=
+  differ_pointwise (fst s) (fst t) i /\
+  UnderThreadStep (fst s i) ev (fst t i) /\
+  match ev with
+  | Some ev => spec.(Step) (snd s) (i, ev) (snd t)
+  | None => True
+  end.
 
-Lemma eqbEql {i} : eqb i i = true.
-induction i.
-easy.
-simpl.
-easy.
-Qed.
+Definition InterOStep {E F : ESig} {spec : Spec E} (impl : Impl E F) (i : ThreadName)
+  (s : InterState F spec)
+  (ev : Event F)
+  (t : InterState F spec) :=
+  differ_pointwise (fst s) (fst t) i /\
+  OverThreadStep impl (fst s i) ev (fst t i).
 
-Lemma updThsEql {A ths i st} : @updThs A ths i st i = st.
-unfold updThs.
-rewrite eqbEql.
-easy.
-Qed.
-
-Inductive InterStep {E F : ESig} {spec : Spec E} {impl : Impl E F} (i : ThreadName) :
-    InterState -> ThreadLEvent E F -> InterState -> Prop :=
-    | IOCall ths st R m :
-        ths i = Idle ->
-        InterStep i (ths, st) (i, OCallEv m) (updThs ths i (Cont m (impl R m)), st)
-    | IORet ths st R m n :
-        ths i = Cont m (Return n) ->
-        InterStep i (ths, st) (i, ORetEv (Ret := R) m n) (updThs ths i Idle, st)
-    | IUCall ths st A (m : E A) R (m' : F R) k st' :
-        ths i = Cont m' (Bind m k) ->
-        spec.(Step) st (i, CallEv m) st' ->
-        InterStep i (ths, st) (i, UCallEv m) (updThs ths i (UCall m' k), st')
-    | IURet ths st A m (n : A) R m' k st' : 
-        ths i = UCall (Ret := R) m' k ->
-        spec.(Step) st (i, RetEv m n) st' -> 
-        InterStep i (ths, st) (i, URetEv m n) (updThs ths i (Cont m' (k n)), st')
-    | IUSilent ths st R m (p : _ R) :
-        ths i = Cont m (NoOp p) ->
-        InterStep i (ths, st) (i, Silent) (updThs ths i (Cont m p), st).
-
-Definition ImplSteps i {E F : ESig} {spec : Spec E} {impl : Impl E F} : 
-    InterState (spec := spec) -> Trace (ThreadLEvent E F) -> InterState -> Prop := 
-        Steps (fun thst ev thst' => InterStep (impl := impl) i thst ev thst').
-
-Definition InterSteps {E F : ESig} {spec : Spec E} {impl : Impl E F} : 
-    InterState (spec := spec) -> Trace (ThreadLEvent E F) -> InterState -> Prop := 
-        Steps (fun thst ev thst' => exists i, InterStep (impl := impl) i thst ev thst').
-
-Definition IsTraceOfInter {E F : ESig} (t : Trace (ThreadLEvent E F)) (lay : Layer E F) := 
-    exists thst, IsPathOf (allIdle, lay.(USpec).(Init)) t thst (InterSteps (impl := lay.(LImpl))).
-
-Definition IsTraceOfInterOv {E F : ESig} (t : Trace (ThreadEvent F)) (lay : @Layer E F) := 
-    exists t', t = projOver t' /\ IsTraceOfInter t' lay.
-
-Inductive InterUStep {E F : ESig} {spec : Spec E} : 
-    InterState (F := F) -> InterState -> Prop :=
-    | InterUCall ths st i A (m : E A) R m' k ths' st' : 
-        ths i = Cont m' (Bind m k) ->
-        ths' i = UCall m' (Ret := R) k ->
-        spec.(Step) st (i, CallEv m) st' ->
-        differ_pointwise ths ths' i -> 
-        InterUStep (ths, st) (ths', st')
-    | InterURet ths st i A m (n : A) R m' k ths' st' : 
-        ths i = UCall (Ret := R) m' k ->
-        ths' i = Cont m' (k n) -> 
-        spec.(Step) st (i, RetEv m n) st' -> 
-        differ_pointwise ths ths' i -> 
-        InterUStep (ths, st) (ths', st')
-    | InterUSilent ths st i R m (p : _ R) ths' :
-        ths i = Cont m (NoOp p) ->
-        ths' i = Cont m p -> 
-        differ_pointwise ths ths' i -> 
-        InterUStep (ths, st) (ths', st).
-
-Definition InterUSteps {E F : ESig} {spec : Spec E} : 
-    InterState (F := F) -> InterState -> Prop := 
-    clos_refl_trans InterState (InterUStep (spec := spec)).
-
-Inductive InterOStep {E F : ESig} {spec : Spec E} {impl : Impl E F} :
-    InterState (spec := spec) -> ThreadLEvent E F -> InterState -> Prop  :=
-    | InterOCall ths st i R m ths' :
-        ths i = Idle -> 
-        ths' i = Cont m (impl R m) ->
-        differ_pointwise ths ths' i -> 
-        InterOStep (ths, st) (i, OCallEv m) (ths', st)
-    | InterORet ths st i R m n ths' :
-        ths i = Cont m (Return n) ->
-        ths' i = Idle -> 
-        differ_pointwise ths ths' i -> 
-        InterOStep (ths, st) (i, ORetEv (Ret := R) m n) (ths', st).
+Definition InterUSteps {E : ESig} F (spec : Spec E) : 
+  InterState F spec -> Trace (option (Event E)) -> InterState F spec -> Prop := 
+  Steps (fun s ev t => exists i, InterUStep i s ev t).
 
 Definition overObj {E F : ESig} (lay : @Layer E F) : Spec F := 
-    {|
-        State := InterState (spec := lay.(USpec));
-        Step thst ev thst'' := exists thst' ev', 
-            InterUSteps thst thst' /\ projOverEv ev' = Some ev /\ InterOStep (impl := lay.(LImpl)) thst' ev' thst'';
-        Init := (allIdle, lay.(USpec).(Init))
-    |}.
+  {|
+    State := InterState F lay.(USpec);
+    Step thst ev thst'' :=
+      exists thst' p,
+        InterUSteps thst p thst' /\
+        InterOStep lay.(LImpl) (fst ev) thst' (snd ev) thst'';
+    Init := (allIdle, lay.(USpec).(Init))
+  |}.
 
 (* Refinement *)
 
 Definition specRefines {E : ESig} (spec : Spec E) (spec': Spec E) : Prop := 
-    Incl (fun t => IsTraceOfSpec t spec) (fun t => IsTraceOfSpec t spec'). 
+  Incl (fun t => IsTraceOfSpec t spec) (fun t => IsTraceOfSpec t spec'). 
 
 Definition layerRefines {E E' F} (lay : @Layer E F) (lay': @Layer E' F)  := 
    specRefines (overObj lay) (overObj lay').
