Util/Tactics.v
@@ -10,3 +10,9 @@ Ltac injpair :=
   subst; injpair_; subst.
 
 Ltac inv H := inversion H; clear H; subst.
+
+Ltac destruct_all :=
+repeat lazymatch goal with
+| [ H : ?P /\ ?Q |- _] => destruct H
+| [ H : exists x, ?P |- _] => destruct H
+end.
